Red2

src/lib/MyLtac2.v
@@ -3,12 +3,11 @@ From Ltac2 Require Option Array Ident Control Std Fresh Message Constr.
 Import Constr.Unsafe.
 
 Ltac2 or t0 t1 :=
-  match! 'True with
-  | True => t0 ()
-  | _ => t1 ()
-  end.
-
-Ltac2 fail () := Control.zero Match_failure.
+  fun x =>
+    match! 'True with
+    | True => t0 x
+    | _ => t1 x
+    end.
 
 Ltac2 Type exn ::= [ TCSearchSuccess (constr) | TCSearchFail ].
 
@@ -16,7 +15,7 @@ Ltac2 evar t n :=
   let u := open_constr:(_: ltac:(exact_no_check $t)) in
   match Constr.Unsafe.kind u with
   | Constr.Unsafe.Cast v _ _ =>
-      Std.pose n t;
+      Std.pose n u;
       v
   | _ => Control.throw Init.Assertion_failure
   end
@@ -35,7 +34,30 @@ Ltac2 unshelve_evar1 e n :=
   (ltac1:(e n|- unshelve evar (n: e))) (Ltac1.of_constr e) (Ltac1.of_ident n)
 .
 
+Ltac2 multiverse_execute tac :=
+  let l := Array.make 1 (None: constr option) in
+  Control.plus
+    (fun _ =>
+       let v := tac () in
+       Array.set l 0 (Some v);
+       Control.zero (Tactic_failure None)
+    )
+    (fun e =>
+       match Array.get l 0 with
+       | Some c => c
+       | None => Control.zero (Tactic_failure None)
+       end).
+
 Ltac2 tcsearch e :=
+  multiverse_execute
+    (fun _ =>
+       let n := Fresh.in_goal ident:(_TC_) in
+       unshelve_evar e n > [|typeclasses_eauto];
+       Std.eval_unfold [(Std.VarRef n, Std.AllOccurrences)] (Control.hyp n)).
+
+(* the one below seems more natural, but it doesn't work as intended. *)
+(* I don't know why... *)
+Ltac2 tcsearch_alt e :=
   Control.plus
     (fun _ =>
        let n := Fresh.in_goal ident:(_TC_) in
@@ -51,16 +73,24 @@ Ltac2 tcsearch e :=
     )
 .
 
-Module _TEST.
+Module TEST.
+  Variable A: Type.
+  Variable a b: A.
+
   Class Foo (n: nat) := mk_Foo {}.
   Global Instance foo: Foo 3 := mk_Foo _.
 
+  Class Bar (a: A) := mk_Bar { Bar_contents: A; }.
+
+  Instance bar: Bar a := mk_Bar _ b.
+
   Goal True.
-    time (do 100 (let _ := tcsearch constr:(Foo 3) in ())).
+    time (let _ := tcsearch_alt constr:(Foo 3) in ()).
+    Fail (let _ := tcsearch_alt constr:(Bar a) in ()). (* why? *)
+    time (do 100 (let _ := tcsearch constr:(Bar a) in ())).
     exact I.
   Qed.
-End _TEST.
-
+End TEST.
 
 Ltac message :=
   ltac2:(e |-
