src/lib/Red2.v
@@ -10,9 +10,26 @@ Ltac2 ctx_rw p :=
   let x := open_constr:(_) in
   let c := Std.eval_hnf open_constr:($p $x) in
   Std.unify c (Control.goal ());
-  refine (open_constr:(@eq_rw _ $p $x _ _ _)) >
+  Control.refine (fun _ => open_constr:(@eq_rw _ $p $x _ _ _)) >
     [Control.shelve ()| |hnf].
 
+(* Internals *)
+Lemma _equal_f (A B : Type) (f g : A -> B)
+      x
+      (EQ: f = g)
+  :
+    f x = g x.
+Proof.
+  subst. apply @eq_refl.
+Qed.
+
+Lemma _einit (P Q: Prop)
+      (EQ: P = Q)
+  :
+    Q -> P.
+Proof.
+  subst. eapply @id.
+Qed.
 
 Variant red_class: Type := | red_class_cons: string -> red_class.
 
@@ -39,8 +56,7 @@ Arguments red_db_incl_next [_] _.
 Ltac2 rec _red_tac c term k :=
   match c with
   | Some c =>
-      or (fun _ =>
-            let tc := tcsearch constr:(@red_db $c _ $term) in
+      first[let tc := tcsearch constr:(@red_db $c _ $term) in
             let lem := (Std.eval_red (Std.eval_red constr:(red_lemma $tc))) in
             let focused := (Std.eval_red (Std.eval_red constr:(red_focused $tc))) in
             let next := (Std.eval_red (Std.eval_red constr:(red_next $tc))) in
@@ -48,11 +64,11 @@ Ltac2 rec _red_tac c term k :=
                         | inr ?next => Some constr:($next)
                         | inl _ => None
                         end in
-            _red_tac next focused (fun _ => k; eapply $lem))
-         (fun _ =>
-            let tc := tcsearch constr:(@red_db_incl $c) in
+            _red_tac next focused (fun _ => k (); (eapply $lem))
+           |let tc := tcsearch constr:(@red_db_incl $c) in
             let next := (Std.eval_red (Std.eval_red constr:(red_db_incl_next $tc))) in
-            _red_tac (Some next) term k)
+            _red_tac (Some next) term k
+        ]
   | None =>
       k ()
   end.
@@ -106,774 +122,42 @@ Module TUTORIAL.
 
     Instance cl_B_unfold_cl_B: red_db_incl cl_B := mk_red_db_incl _ cl_B_unfold.
 
-    (* Instance cl_B_unfold_cl_B: red_db_incl cl_B_unfold cl_B := mk_red_db_incl. *)
-
     Instance foo_red_f_hint a: red_db cl_B (f a) :=
-      mk_red_db _ _ (@f_equal _ _ f) a (inr cl_B).
+      mk_red_db _ _ (@f_equal _ _ f) a (inr cl_B_unfold).
 
+    Ltac2 rec __ctx n :=
+      if (Int.le n 0)
+      then (eapply f_equal)
+      else (eapply _equal_f; __ctx (Int.sub n 1)).
 
-    Class Foo (n: nat) := mk_Foo {}.
-    Global Instance foo: Foo 3 := mk_Foo _.
+    Ltac2 rec _ctx l :=
+      match l with
+      | hd::tl => __ctx hd; _ctx tl
+      | [] => ()
+      end.
 
+    Ltac2 ctx l :=
+      eapply _einit > [_ctx l|].
 
-    Ltac2 evar t n :=
-      let u := open_constr:(_: ltac:(exact_no_check $t)) in
-      match Constr.Unsafe.kind u with
-      | Constr.Unsafe.Cast v0 _ v1 =>
-          Message.print (Message.of_constr v0);
-          Message.print (Message.of_constr v1);
-          Std.pose n t;
-          v0
-      | _ => Control.throw Init.Assertion_failure
-      end
-    .
-
-    Ltac2 unshelve_evar e n :=
-      let v := evar e (Some n) in
-      match Constr.Unsafe.kind v with
-      | Constr.Unsafe.Evar e _ =>
-          Control.new_goal e
-      | _ => Control.throw Init.Assertion_failure
-      end
-    .
-
-
-    Goal True.
-    Proof.
-
-      let n := Fresh.in_goal ident:(_TC_) in
-      unshelve_evar constr:(nat) n > [|exact 5].
-
-      let e := constr:(red_db cl_A a) in
-      Message.print (Message.of_constr e);
-      Message.print (Message.of_constr constr:(22));
-      let n := Fresh.in_goal ident:(_TC_) in
-      Message.print (Message.of_constr constr:(33));
-      let u := open_constr:(_) in
-      unshelve_evar e n > [|typeclasses_eauto];
-      let x := (TCSearchSuccess (Std.eval_unfold [(Std.VarRef n, Std.AllOccurrences)] (Control.hyp n))) in
-      Message.print (Message.of_constr (Control.hyp n));
-      Message.print (Message.of_constr (Std.eval_unfold [(Std.VarRef n, Std.AllOccurrences)] (Control.hyp n)))
-      .
-
-
-      let n := Fresh.in_goal ident:(_TC_) in
-      Std.pose (Some n) constr:(42);
-
-      Message.print (Message.of_constr (Std.eval_unfold [(Std.VarRef n, Std.AllOccurrences)] (Control.hyp n)));
-      Message.print (Message.of_constr ((Control.hyp n)))
-      .
-
-
-      Std.pose None (Std.eval_unfold [(Std.VarRef n, Std.AllOccurrences)] (Control.hyp n))
-      .
-
-                       (Control.hyp n)).
-
-
-      n.
-
-
-      let a :=
-
-      let e := constr:(red_db cl_A a) in
-      Message.print (Message.of_constr constr:(11));
-      Control.plus
-
-        (fun _ =>
-
-           Message.print (Message.of_constr e);
-           Message.print (Message.of_constr constr:(22));
-
-           let n := Fresh.in_goal ident:(_TC_) in
-           Message.print (Message.of_constr constr:(33));
-           let u := open_constr:(_) in
-           unshelve_evar e n > [|typeclasses_eauto];
-           let x := (TCSearchSuccess (Std.eval_unfold [(Std.VarRef n, Std.AllOccurrences)] (Control.hyp n))) in
-           Message.print (Message.of_constr (Control.hyp n));
-           Message.print (Message.of_constr (Std.eval_unfold [(Std.VarRef n, Std.AllOccurrences)] (Control.hyp n)));
-
-           Message.print (Message.of_constr u);
-           Message.print (Message.of_constr constr:(55));
-           Control.zero (TCSearchSuccess u)
-        )
-
-        (fun e =>
-           Message.print (Message.of_constr constr:(66));
-           Message.print (Message.of_exn e);
-           match e with
-           | TCSearchSuccess c =>
-               Message.print (Message.of_constr constr:(c));
-               c
-           | _ =>
-               constr:(3)
-               (* Control.zero e *)
-           end
-        ).
-
-      or
-        (fun _ =>
-           let e := constr:(red_db cl_A a) in
-           Message.print (Message.of_constr constr:(11));
-
-
-           Control.plus
-
-             (fun _ =>
-
-                Message.print (Message.of_constr constr:(22));
-
-
-                let n := Fresh.in_goal ident:(_TC_) in
-                unshelve_evar e n > [|typeclasses_eauto];
-                Control.zero (TCSearchSuccess (Std.eval_unfold [(Std.VarRef n, Std.AllOccurrences)] (Control.hyp n)))
-             )
-
-             (fun e =>
-                match e with
-                | TCSearchSuccess c =>
-                    c
-                | _ => Control.zero e
-                end
-        ))
-        (fun _ => ()) ()
-      .
-
-
-
-
-Ltac2 evar t n :=
-  let u := open_constr:(_: ltac:(exact_no_check $t)) in
-  match Constr.Unsafe.kind u with
-  | Constr.Unsafe.Cast v _ _ =>
-      Std.pose n t;
-      v
-  | _ => Control.throw Init.Assertion_failure
-  end
-.
-
-Ltac2 unshelve_evar e n :=
-  let v := evar e (Some n) in
-  match Constr.Unsafe.kind v with
-  | Constr.Unsafe.Evar e _ =>
-      Control.new_goal e
-  | _ => Control.throw Init.Assertion_failure
-  end
-.
-
-Ltac2 unshelve_evar1 e n :=
-  (ltac1:(e n|- unshelve evar (n: e))) (Ltac1.of_constr e) (Ltac1.of_ident n)
-.
-
-Ltac2 tcsearch e :=
-  Control.plus
-    (fun _ =>
-       let n := Fresh.in_goal ident:(_TC_) in
-       unshelve_evar e n > [|typeclasses_eauto];
-       Control.zero (TCSearchSuccess (Std.eval_unfold [(Std.VarRef n, Std.AllOccurrences)] (Control.hyp n)))
-    )
-    (fun e =>
-       match e with
-       | TCSearchSuccess c =>
-           c
-       | _ => Control.zero e
-       end
-    )
-.
-
-
-
-      time (do 100 (let _ := tcsearch constr:(red_db cl_A a) in ())).
-
-        let x := tcsearch constr:(red_db cl_A a) in ().
-
-      exact I.
-    Qed.
-
-
+    (* much fast *)
     Goal forall (n: nat) (H: sim c ((n, f z), q) n),
         sim a ((n, f x), p) n.
     Proof.
-
-      Set Ltac Profiling.
       intros n H.
-
-      ctx_rw open_constr:(fun t => _ t _ _).
-      {
-
-        let c := constr:(cl_A) in
-        match! Control.goal () with
-        | ?term = _ =>
-            Message.print (Message.of_constr constr:((@red_db $c _ $term)));
-            let tc := tcsearch constr:(@red_db $c _ $term) in
-            let lem := (Std.eval_red (Std.eval_red constr:(red_lemma $tc))) in
-            let focused := (Std.eval_red (Std.eval_red constr:(red_focused $tc))) in
-            let next := (Std.eval_red (Std.eval_red constr:(red_next $tc))) in
-            let next := match! next with
-                        | inr ?next => Some constr:($next)
-                        | inl _ => None
-                        end in
-            _red_tac next focused (fun () => eapply $lem)
-        | _ =>
-            Message.print (Message.of_int 999)
-        end.
-
-
-        let x := tcsearch constr:(red_db cl_A a) in ().
-
-
-
-
-  match c with
-  | Some c =>
-      or (fun _ =>
-            let tc := tcsearch constr:(@red_db $c _ $term) in
-            let lem := (Std.eval_red (Std.eval_red constr:(red_lemma $tc))) in
-            let focused := (Std.eval_red (Std.eval_red constr:(red_focused $tc))) in
-            let next := (Std.eval_red (Std.eval_red constr:(red_next $tc))) in
-            let next := match! next with
-                        | inr ?next => Some constr:($next)
-                        | inl _ => None
-                        end in
-            _red_tac next focused (fun _ => k; eapply $lem))
-         (fun _ =>
-            let tc := tcsearch constr:(@red_db_incl $c) in
-            let next := (Std.eval_red (Std.eval_red constr:(red_db_incl_next $tc))) in
-            _red_tac (Some next) term k)
-  | None =>
-      k ()
-  end.
-
-        let c := constr:(cl_A) in
-        match! Control.goal () with
-        | ?term = _ =>
-            (_red_tac (Some c) term (fun _ => ()))
-        | _ =>
-            Message.print (Message.of_int 999)
-        end.
-
-
-        red_tac constr:(cl_A).
-
-
-        match! goal with
-        | [ |- ?term = _ ] =>
-            (_red_tac (Some c) term (fun _ => ()))
-        end.
-
-
-        red_tac constr:(cl_A).
-
-
-      try (prw ltac:(red_tac cl_A) 3 0).
-      Show Proof.
-
-      ltac2:(open_constr:(_ : ltac:(exact_no_check $type))).
-
-      (prw ltac:(red_tac cl_C) 2 1 0).
-      (prw ltac:(red_tac cl_B) 2 2 1 0).
-      exact H.
-      Show Ltac Profile.
-    Qed.
-
-  End FOO.
-End TUTORIAL.
-
-
-
-Module TUTORIAL.
-  Section FOO.
-    (* Variables *)
-    Variable A B C: Type.
-    Variable a b c d: A.
-    Variable x y z: B.
-    Variable p q: C.
-
-    Variable sim: A -> (nat * B) * C -> nat -> Prop.
-
-    (* First Step: Prove Reduction Lemmas *)
-    Hypothesis foo_red0: a = b.
-    Hypothesis foo_red1: b = c.
-    Hypothesis foo_red2: c = d.
-    Hypothesis foo_red3: x = y.
-    Hypothesis foo_red4: y = z.
-    Hypothesis foo_red5: p = q.
-
-    (* Second Step: Define Reduction Strategy (= red_tac) *)
-    Ltac red_A f := (* f is a flag indicating continue/break/fail. Must set f before return *)
-      ((apply foo_red0; fail) ||
-       (apply foo_red1; fail) ||
-       (apply foo_red2; fail)).
-
-    (* We also give more conenient syntax *)
-    Ltac red_A' := (* = red_A *)
-      rwal (foo_red0, _continue)
-           (foo_red1, _break)
-           (foo_red2, _break)
-           0.
-
-    Ltac red_B :=
-      rwcl foo_red3
-           foo_red4
-           0.
-
-    Ltac red_B' f := (* = red_B *)
-      ((instantiate (f:=_continue); apply foo_red3; fail) ||
-       (instantiate (f:=_continue); apply foo_red4; fail)).
-
-    Ltac red_C :=
-      rrw foo_red5 _break.
-
-    Ltac red_C' := (* = red_C *)
-      rwbl
-        foo_red5
-        0.
-
-    Ltac red_C'' f := (* = red_C *)
-      (instantiate (f:=_break); apply foo_red5; fail).
-
-    (* Done. Let's use it! *)
-    Lemma foo: forall (n: nat) (H: sim c ((n, z), q) n),
-        sim a ((n, x), p) n.
-    Proof.
-      intros n H.
-      (* goal = sim a (n, x, p) n *)
-      prw red_B 2 2 1 0.
-      (* prw [red_tac (= red_r)] [l_0 (= 2)] [l_1 (= 2)] [l_2 (= 1)] ... 0 =>
-         - find the right l_0th term x0 (= ((n, x), p)) in the goal
-         - find the right l_1th term x1 (=  (n, x)    ) in the   x0
-         - find the right l_2th term x2 (=      x     ) in the   x1
-         ...
-         - the last argument must be 0. reduce the x2 following _red_r *)
-      (* goal = sim a (n, z, p) n *)
-      prw red_A 3 0.
-      (* goal = sim c (n, z, p) n *)
-      prw red_C 2 1 0.
-      (* goal = sim c (n, z, q) n *)
+      do 2 (ctx [2] > [red_tac constr:(cl_A)|]);
+      do 1 (ctx [1; 0] > [red_tac constr:(cl_C)|]);
+      do 2 (ctx [1; 1; 0] > [red_tac constr:(cl_B)|]);
       exact H.
     Qed.
-  End FOO.
-End TUTORIAL.
 
-
-(* Ltac2 ctx_rw p := *)
-(*   let x := open_constr:(_) in *)
-(*   let c := Std.eval_hnf open_constr:($p $x) in *)
-(*   Std.unify c (Control.goal ()); *)
-(*   refine (open_constr:(@eq_rect_r _ _ $p _ $x _)) > *)
-(*     [Control.shelve ()|hnf|]. *)
-
-
-(* Ltac2 __prw red_tac success := *)
-(*   cbn; *)
-(*   tryif (let f := fresh "f" in *)
-(*          evar (f:_flag); *)
-(*          etransitivity; *)
-(*          [red_tac| *)
-(*            match goal with *)
-(*            | [f0:= ?f1: _flag|- _] => *)
-(*                match f1 with *)
-(*                | _continue => subst f; __prw red_tac true *)
-(*                | _break => subst f; reflexivity *)
-(*                | _fail => fail 2 *)
-(*                end *)
-(*            end]) *)
-(*   then *)
-(*     idtac *)
-(*   else *)
-(*     match success with *)
-(*     | true => reflexivity *)
-(*     | false => fail *)
-(*     end. *)
-
-Class Foo (n: nat) := mk_Foo {}.
-Instance foo: Foo 3 := mk_Foo _.
-
-Import Constr.Binder Constr.Unsafe.
-
-Goal forall X Y (f: X -> Y) (x: X) (y: Y), f x = y.
-Proof.
-  intros.
-
-  Show Proof.
-
-  let p := open_constr:(fun t => _ t = _) in
-  let x := open_constr:(_) in
-  let c := Std.eval_hnf open_constr:($p $x) in
-  Std.unify c (Control.goal ());
-  refine (open_constr:(@eq_rw _ $p $x _ _ _)) >
-    [Control.shelve ()| |hnf].
-
-
-  ctx_rw open_constr:(fun t => _ t = _).
-  Show Proof.
-
-  let p := open_constr:(fun t => _ t = _) in
-  let x := open_constr:(_) in
-  let c := Std.eval_hnf open_constr:($p $x) in
-  Std.unify c (Control.goal ());
-  refine (open_constr:(@eq_rect_r _ _ $p _ $x _)) >
-    [Control.shelve ()|hnf|].
-
-
-  (let p := open_constr:(fun t => _ t = _) in
-   let x := open_constr:(_) in
-   let c := Std.eval_hnf open_constr:($p $x) in
-   Std.unify c (Control.goal ());
-   (Control.refine (fun _ => open_constr:(@eq_rect_r _ _ $p _ $c _)))).
-
-
-  >
-    [pose 0|pose 1|pose 2|pose 3|pose 4|pose 5|pose 6].
-
-  Control.shelve().
-  Control.shelve().
-  hnf.
-
-
-  > [Control.shelve()|..])).
-
-
-  let p := open_constr:(fun t => _ t = _) in
-  let x := open_constr:(_) in
-  let c := Std.eval_hnf open_constr:($p $x) in
-  Std.unify c (Control.goal ());
-  refine (open_constr:(@eq_rect_r _ _ $p _ $x _)) >
-    [Control.shelve ()|hnf|].
-
-
-
-  (let p := open_constr:(fun t => _ t = _) in
-   let x := open_constr:(_) in
-   (Control.refine (fun _ => open_constr:(@eq_rect_r _ _ $p _ $x _)) > [Control.shelve()|..])).
-
-  Control.shelve ().
-                                                  hnf.
-
-  >
-    [Control.shelve ()|hnf|].
-
-
-  time (let p := open_constr:(fun t => _ t = _) in
-        let x := open_constr:(_) in
-        let c := Std.eval_hnf open_constr:($p $x) in
-        Std.unify c (Control.goal ());
-        refine (open_constr:(@eq_rect_r _ _ $p _ $x _)) >
-          [Control.shelve ()|hnf|]).
-
-Show Proof.
-
-  let c := open_constr:(@eq_rect_r _ _ $x _ _ _) in
-  eapply $c.
-
-  Show Proof.
-
-
- _ _ _)
-  .
-
-
-  let u := open_constr:(_: ltac:(exact_no_check $t)) in
-  match Constr.Unsafe.kind u with
-  | Constr.Unsafe.Cast v _ _ =>
-      let f := open_constr:(fun _t => _ _t = _) in
-      Std.unify open_constr:($f _) (Control.goal ());
-      Std.pose None f
-      v
-  | _ => Control.throw Init.Assertion_failure
-  end
-  .
-
-
-  .
-
-
-  let n := Fresh.in_goal ident:(x) in
-  let b := Constr.Binder.make (Some n) open_constr:(X) in
-  let x := Constr.Unsafe.make (Constr.Unsafe.Rel 1) in
-  let a := Constr.Unsafe.make (Constr.Unsafe.Lambda b open_constr:(_ $x = _)) in
-  Std.unify constr:($a x) (Control.goal ());
-  Std.pose None a
-  .
-
-  end.
-
- =>
-                                 match (Constr.Unsafe.kind c) with
-                                 | Rel n
-                                   => Message.print (Message.of_int n)
-
-
-open_constr:(fun _t => _ _t = _) in
-  Std.unify constr:($a x) (Control.goal ());
-  Std.pose None a
-  .
-
-
-  match (Constr.Unsafe.kind constr:(fun x: nat => x)) with
-  | Constr.Unsafe.Lambda b c =>
-      match (Constr.Unsafe.kind c) with
-      | Rel n
-        => Message.print (Message.of_int n)
-
-
-
-
-    (* | Var _ *)
-      (*   => Message.print (Message.of_string "1") *)
-      (* | Meta _ *)
-      (*   => Message.print (Message.of_string "2") *)
-      (* | Evar _ _ *)
-      (*   => Message.print (Message.of_string "3") *)
-      (* | Sort _ *)
-      (*   => Message.print (Message.of_string "4") *)
-      (* | Cast _ _ _ *)
-      (*   => Message.print (Message.of_string "5") *)
-      (* | Prod _ _ *)
-      (*   => Message.print (Message.of_string "6") *)
-      (* | Lambda _ _ *)
-      (*   => Message.print (Message.of_string "7") *)
-      (* | LetIn _ _ _ *)
-      (*   => Message.print (Message.of_string "8") *)
-      (* | App _ _ *)
-      (*   => Message.print (Message.of_string "9") *)
-      (* | Constant _ _ *)
-      (*   => Message.print (Message.of_string "10") *)
-      (* | Ind _ _ *)
-      (*   => Message.print (Message.of_string "11") *)
-      (* | Constructor _ _ *)
-      (*   => Message.print (Message.of_string "12") *)
-      (* | Case _ _ _ _ _ *)
-      (*   => Message.print (Message.of_string "13") *)
-      (* | Fix _ _ _ _ *)
-      (*   => Message.print (Message.of_string "14") *)
-      (* | CoFix _ _ _ *)
-      (*   => Message.print (Message.of_string "15") *)
-      (* | Proj _ _ *)
-      (*   => Message.print (Message.of_string "16") *)
-      (* | Uint63 _ *)
-      (*   => Message.print (Message.of_string "17") *)
-      (* | Float _ *)
-      (*   => Message.print (Message.of_string "18") *)
-      (* | Array _ _ _ _ *)
-      (*   => Message.print (Message.of_string "19") *)
-      | _ => Control.throw Init.Assertion_failure
-      end
-  | _ => Control.throw Init.Assertion_failure
-  end
-  .
-
-
-Some c =>
-      let c := Constr.Unsafe.make (Constr.Unsafe.Var c) in
-      let a := Constr.Unsafe.make (Constr.Unsafe.Lambda b open_constr:(_ $c = _)) in
-      Std.unify constr:($a x) (Control.goal ());
-      Std.pose None a
-  | _ => Control.throw Init.Assertion_failure
-  end
-  .
-
-
-
-
-  let n := Fresh.in_goal ident:(_TC_) in
-  let b := Constr.Binder.make (Some n) constr:(X) in
-  match (Constr.Binder.name b) with
-  | Some c =>
-      let c := Constr.Unsafe.make (Constr.Unsafe.Var c) in
-      let a := Constr.Unsafe.make (Constr.Unsafe.Lambda b open_constr:(_ $c = _)) in
-      Std.unify constr:($a x) (Control.goal ());
-      Std.pose None a
-  | _ => Control.throw Init.Assertion_failure
-  end
-  .
-
-  let a := open_constr:(fun _t => _ _t = _) in
-  Std.unify constr:($a x) (Control.goal ());
-  Std.pose None a
-  .
-
-
-  let n := Fresh.in_goal ident:(_TC_) in
-  let b := Constr.Binder.make (Some n) constr:(X) in
-  match (Constr.Binder.name b) with
-  | Some c =>
-      let c := Constr.Unsafe.make (Constr.Unsafe.Var c) in
-      let a := Constr.Unsafe.make (Constr.Unsafe.Lambda b open_constr:(_ $b = _)) in
-      Std.unify constr:($a x) (Control.goal ());
-      Std.pose None a
-  | _ => Control.throw Init.Assertion_failure
-  end
-  .
-
-
- ().
-
-
-  let n := Fresh.in_goal ident:(_TC_) in
-  let a := open_constr:(fun $n => _ $n = _) in
-  Std.unify constr:($a x) (Control.goal ());
-  Std.pose None a
-  .
-  Show Proof.
-
-  let n := Fresh.in_goal ident:(_TC_) in
-  Std.in_context
-
-
-
-Goal False.
-Proof.
-  assert (Foo 3).
-  { pose foo.
-
-let n := Fresh.in_goal ident:(_TC_) in
-    let m := (Constr.in_context n constr:(unit) (fun _ => typeclasses_eauto)) in
-    Message.print (Message.of_constr m).
-
-
-Message.print (mes.
-
-
-
-
-Ltac2 @ external in_context : ident -> constr -> (unit -> unit) -> constr := "coq-core.plugins.ltac2" "constr_in_context".
-(** On a focused goal [Γ ⊢ A], [in_context id c tac] evaluates [tac] in a
-    focused goal [Γ, id : c ⊢ ?X] and returns [fun (id : c) => t] where [t] is
-    the proof built by the tactic. *)
-
-  intros.
-  Std.unify
-
-
-Ltac2 rec holes pos :=
-  match pos with
-  | hd::tl =>
-      if (Int.le hd 0)
-      then
-        let k := holes tl in
-        open_constr:($k _)
-      else
-        holes tl
-  | [] =>
-      open_constr:(4)
-  end.
-
-
-
-
-open_constr:(_: ltac:(exact_no_check $t))
-
-                       |
-
-
-  if (Int.le n 0)
-  then
-    (apply f_equal)
-  else
-    (apply _equal_f; _ctx (Int.sub n 1))
-
-
-  match n with
-  |
-
-  match holes with
-  | hd::tl =>
-
-Ltac2 rec holes pos :=
-  match holes with
-  | hd::tl =>
-
-
-Ltac2 evar t n :=
-  let u := open_constr:(_: ltac:(exact_no_check $t)) in
-  match Constr.Unsafe.kind u with
-  | Constr.Unsafe.Cast v _ _ =>
-      Std.pose n t;
-      v
-  | _ => Control.throw Init.Assertion_failure
-  end
-.
-
-Ltac2 _prw k0 k1 X :=
-  match X with
-  | O => eapply _einit > [(k0; k1)|]
-  | S ?n => _prw ltac:(k0; _ctx n) k1
-  end.
-
-(* Main Tactic *)
-Ltac prw red_tac X := _prw ltac:(idtac) ltac:(__prw red_tac false) X.
-
-Module TUTORIAL.
-  Section FOO.
-    (* Variables *)
-    Variable A B C: Type.
-    Variable a b c d: A.
-    Variable x y z: B.
-    Variable p q: C.
-
-    Variable sim: A -> (nat * B) * C -> nat -> Prop.
-
-    (* First Step: Prove Reduction Lemmas *)
-    Hypothesis foo_red0: a = b.
-    Hypothesis foo_red1: b = c.
-    Hypothesis foo_red2: c = d.
-    Hypothesis foo_red3: x = y.
-    Hypothesis foo_red4: y = z.
-    Hypothesis foo_red5: p = q.
-
-    (* Second Step: Define Reduction Strategy (= red_tac) *)
-    Ltac red_A f := (* f is a flag indicating continue/break/fail. Must set f before return *)
-      ((instantiate (f:=_continue); apply foo_red0; fail) ||
-       (instantiate (f:=_break); apply foo_red1; fail) ||
-       (instantiate (f:=_fail); apply foo_red2; fail)).
-
-    (* We also give more conenient syntax *)
-    Ltac red_A' := (* = red_A *)
-      rwal (foo_red0, _continue)
-           (foo_red1, _break)
-           (foo_red2, _break)
-           0.
-
-    Ltac red_B :=
-      rwcl foo_red3
-           foo_red4
-           0.
-
-    Ltac red_B' f := (* = red_B *)
-      ((instantiate (f:=_continue); apply foo_red3; fail) ||
-       (instantiate (f:=_continue); apply foo_red4; fail)).
-
-    Ltac red_C :=
-      rrw foo_red5 _break.
-
-    Ltac red_C' := (* = red_C *)
-      rwbl
-        foo_red5
-        0.
-
-    Ltac red_C'' f := (* = red_C *)
-      (instantiate (f:=_break); apply foo_red5; fail).
-
-    (* Done. Let's use it! *)
-    Lemma foo: forall (n: nat) (H: sim c ((n, z), q) n),
-        sim a ((n, x), p) n.
+    (* more flexible and easy to use, but slow *)
+    Goal forall (n: nat) (H: sim c ((n, f z), q) n),
+        sim a ((n, f x), p) n.
     Proof.
       intros n H.
-      (* goal = sim a (n, x, p) n *)
-      prw red_B 2 2 1 0.
-      (* prw [red_tac (= red_r)] [l_0 (= 2)] [l_1 (= 2)] [l_2 (= 1)] ... 0 =>
-         - find the right l_0th term x0 (= ((n, x), p)) in the goal
-         - find the right l_1th term x1 (=  (n, x)    ) in the   x0
-         - find the right l_2th term x2 (=      x     ) in the   x1
-         ...
-         - the last argument must be 0. reduce the x2 following _red_r *)
-      (* goal = sim a (n, z, p) n *)
-      prw red_A 3 0.
-      (* goal = sim c (n, z, p) n *)
-      prw red_C 2 1 0.
-      (* goal = sim c (n, z, q) n *)
-      exact H.
+      do 2 (ctx_rw open_constr:(fun t => _ t _ _) > [red_tac constr:(cl_A)|]);
+      do 1 (ctx_rw open_constr:(fun t => sim _ (_, _, t) _) > [red_tac constr:(cl_C)|]);
+      do 2 (ctx_rw open_constr:(fun t => sim _ (_, t, _) _) > [red_tac constr:(cl_B)|]); exact H.
     Qed.
   End FOO.
 End TUTORIAL.
