src/logic/WeakestRed.v
@@ -1,0 +1,4 @@
+From Fairness Require Export LinkingRed.
+
+Ltac lred2 := (prw ltac:(red_tac itree_class) 1 2 0).
+Ltac rred2 := (prw ltac:(red_tac itree_class) 1 1 0).
